weaken path_intro and beta expansion/reduction lemmas by strengthening assumptions

dsn/Lang/Dynamic/Typing.lean
@@ -2,8 +2,7 @@ import Lang.Basic
 import Lang.Dynamic.EvalCon
 import Lang.Dynamic.Transition
 import Lang.Dynamic.TransitionStar
-import Lang.Dynamic.Convergent
-import Lang.Dynamic.Divergent
+import Lang.Dynamic.Safe
 import Lang.Dynamic.FinTyping
 
 set_option pp.fieldNotation false
@@ -37,7 +36,7 @@ mutual
 
   def Typing (am : List (String × Typ)) (e : Expr) : Typ → Prop
   | .bot => False
-  | .top => Convergent e ∨ Divergent e
+  | .top => Safe e
   | .iso l t => Typing am (.extract e l) t
   | .entry l t => Typing am (.project e l) t
   | .path left right => ∀ e' , Typing am e' left → Typing am (.app e e') right
@@ -604,9 +603,10 @@ theorem Typing.path_determines_function
 
 
 
--- theorem Typing.soundness
---   (typing : Typing am e t)
--- : Convergent e ∨ Divergent e
+theorem Typing.soundness
+  (typing : Typing am e t)
+: Safe e
+:= by sorry
 -- := by cases t with
 -- | bot =>
 --   unfold Typing at typing
@@ -1597,7 +1597,7 @@ theorem Subtyping.list_typ_diff_elim :
 mutual
   theorem Typing.function_beta_reduction
     (econ : EvalCon E)
-    (isval : Expr.is_value ev)
+    (safe : Safe ev)
     (matching : Expr.pattern_match ev p = .some eam)
   : Typing am (E (Expr.app (Expr.function ((p, e) :: f)) ev)) t →
     Typing am (E (Expr.sub eam e)) t
@@ -1608,31 +1608,25 @@ mutual
   | top =>
     unfold Typing
     intro h0
-    cases h0 with
-    | inl h1 =>
-      apply Or.inl
-      exact Convergent.function_beta_reduction econ isval matching h1
-    | inr h1 =>
-      apply Or.inr
-      exact Divergent.function_beta_reduction econ isval matching h1
+    exact Safe.function_beta_reduction econ safe matching h0
   | iso label body =>
     unfold Typing
     intro h0
     apply EvalCon.extract label at econ
-    apply Typing.function_beta_reduction econ isval matching h0
+    apply Typing.function_beta_reduction econ safe matching h0
 
   | entry label body =>
     unfold Typing
     intro h0
     apply EvalCon.project label at econ
-    apply Typing.function_beta_reduction econ isval matching h0
+    apply Typing.function_beta_reduction econ safe matching h0
 
   | path left right =>
     unfold Typing
     intro h0 e' h1
     specialize h0 e' h1
     apply EvalCon.applicator e' at econ
-    apply Typing.function_beta_reduction econ isval matching h0
+    apply Typing.function_beta_reduction econ safe matching h0
 
   | unio left right =>
     unfold Typing
@@ -1640,30 +1634,30 @@ mutual
     cases h0 with
     | inl h1 =>
       apply Or.inl
-      apply Typing.function_beta_reduction econ isval matching h1
+      apply Typing.function_beta_reduction econ safe matching h1
 
     | inr h1 =>
       apply Or.inr
-      apply Typing.function_beta_reduction econ isval matching h1
+      apply Typing.function_beta_reduction econ safe matching h1
 
   | inter left right =>
     unfold Typing
     intro h0
     have ⟨h1,h2⟩ := h0
     apply And.intro
-    { apply Typing.function_beta_reduction econ isval matching h1 }
-    { apply Typing.function_beta_reduction econ isval matching h2 }
+    { apply Typing.function_beta_reduction econ safe matching h1 }
+    { apply Typing.function_beta_reduction econ safe matching h2 }
 
   | diff left right =>
     unfold Typing
     intro h0
     have ⟨h1,h2⟩ := h0
     apply And.intro
-    { apply Typing.function_beta_reduction econ isval matching h1 }
+    { apply Typing.function_beta_reduction econ safe matching h1 }
     {
       intro h3
       apply h2
-      apply Typing.function_beta_expansion f econ isval matching h3
+      apply Typing.function_beta_expansion f econ safe matching h3
     }
 
   | exi ids quals body =>
@@ -1673,7 +1667,7 @@ mutual
     exists am'
     apply And.intro h1
     apply And.intro h2
-    apply Typing.function_beta_reduction econ isval matching h3
+    apply Typing.function_beta_reduction econ safe matching h3
 
   | all ids quals body =>
     unfold Typing
@@ -1682,7 +1676,7 @@ mutual
     {
       intro am' dom_subset dynamic_quals
       specialize h0 am' dom_subset dynamic_quals
-      apply Typing.function_beta_reduction econ isval matching h0
+      apply Typing.function_beta_reduction econ safe matching h0
     }
     { exact h1 }
 
@@ -1693,18 +1687,18 @@ mutual
     exists t
     exists lt_size
     apply And.intro imp_typing
-    apply Typing.function_beta_reduction econ isval matching typing_body
+    apply Typing.function_beta_reduction econ safe matching typing_body
 
   | var id =>
     unfold Typing
     intro ⟨t, h1, h2⟩
     exists t
     apply And.intro h1
-    apply FinTyping.function_beta_reduction econ isval matching h2
+    apply FinTyping.function_beta_reduction econ safe matching h2
 
   theorem Typing.function_beta_expansion f
     (econ : EvalCon E)
-    (isval : Expr.is_value ev)
+    (safe : Safe ev)
     (matching : Expr.pattern_match ev p = .some eam)
   : Typing am (E (Expr.sub eam e)) t →
     Typing am (E (Expr.app (Expr.function ((p, e) :: f)) ev)) t
@@ -1715,31 +1709,26 @@ mutual
   | top =>
     unfold Typing
     intro h0
-    cases h0 with
-    | inl h1 =>
-      apply Or.inl
-      exact Convergent.function_beta_expansion f econ isval matching h1
-    | inr h1 =>
-      apply Or.inr
-      exact Divergent.function_beta_expansion f econ isval matching h1
+    exact Safe.function_beta_expansion f econ safe matching h0
+
   | iso label body =>
     unfold Typing
     intro h0
     apply EvalCon.extract label at econ
-    apply Typing.function_beta_expansion f econ isval matching h0
+    apply Typing.function_beta_expansion f econ safe matching h0
 
   | entry label body =>
     unfold Typing
     intro h0
     apply EvalCon.project label at econ
-    apply Typing.function_beta_expansion f econ isval matching h0
+    apply Typing.function_beta_expansion f econ safe matching h0
 
   | path left right =>
     unfold Typing
     intro h0 e' h1
     specialize h0 e' h1
     apply EvalCon.applicator e' at econ
-    apply Typing.function_beta_expansion f econ isval matching h0
+    apply Typing.function_beta_expansion f econ safe matching h0
 
   | unio left right =>
     unfold Typing
@@ -1747,30 +1736,30 @@ mutual
     cases h0 with
     | inl h1 =>
       apply Or.inl
-      apply Typing.function_beta_expansion f econ isval matching h1
+      apply Typing.function_beta_expansion f econ safe matching h1
 
     | inr h1 =>
       apply Or.inr
-      apply Typing.function_beta_expansion f econ isval matching h1
+      apply Typing.function_beta_expansion f econ safe matching h1
 
   | inter left right =>
     unfold Typing
     intro h0
     have ⟨h1,h2⟩ := h0
     apply And.intro
-    { apply Typing.function_beta_expansion f econ isval matching h1 }
-    { apply Typing.function_beta_expansion f econ isval matching h2 }
+    { apply Typing.function_beta_expansion f econ safe matching h1 }
+    { apply Typing.function_beta_expansion f econ safe matching h2 }
 
   | diff left right =>
     unfold Typing
     intro h0
     have ⟨h1,h2⟩ := h0
     apply And.intro
-    { apply Typing.function_beta_expansion f econ isval matching h1 }
+    { apply Typing.function_beta_expansion f econ safe matching h1 }
     {
       intro h3
       apply h2
-      apply Typing.function_beta_reduction econ isval matching h3
+      apply Typing.function_beta_reduction econ safe matching h3
     }
 
   | exi ids quals body =>
@@ -1780,7 +1769,7 @@ mutual
     exists am'
     apply And.intro h1
     apply And.intro h2
-    apply Typing.function_beta_expansion f econ isval matching h3
+    apply Typing.function_beta_expansion f econ safe matching h3
 
   | all ids quals body =>
     unfold Typing
@@ -1789,7 +1778,7 @@ mutual
     {
       intro am' dom_subset dynamic_quals
       specialize h0 am' dom_subset dynamic_quals
-      apply Typing.function_beta_expansion f econ isval matching h0
+      apply Typing.function_beta_expansion f econ safe matching h0
     }
     { exact h1 }
 
@@ -1800,14 +1789,14 @@ mutual
     exists t
     exists lt_size
     apply And.intro imp_typing
-    apply Typing.function_beta_expansion f econ isval matching typing_body
+    apply Typing.function_beta_expansion f econ safe matching typing_body
 
   | var id =>
     unfold Typing
     intro ⟨t, h1, h2⟩
     exists t
     apply And.intro h1
-    apply FinTyping.function_beta_expansion f econ isval matching h2
+    apply FinTyping.function_beta_expansion f econ safe matching h2
 
 
 end
@@ -1833,9 +1822,9 @@ end
 
 
 theorem Typing.path_intro :
-  (∀ {v} ,
-    Expr.is_value v → Typing am v tp →
-    ∃ eam , Expr.pattern_match v p = .some eam ∧ Typing am (Expr.sub eam e) tr
+  (∀ e' ,
+    Typing am e' tp →
+    ∃ eam , Expr.pattern_match e' p = .some eam ∧ Typing am (Expr.sub eam e) tr
   ) →
   Typing am (Expr.function ((p, e) :: f)) (Typ.path (List.typ_diff tp subtras) tr)
 := by
@@ -1843,8 +1832,9 @@ theorem Typing.path_intro :
   unfold Typing
   intro e' h1
   have h2 := Subtyping.elimination Subtyping.list_typ_diff_elim h1
-  sorry
-  -- exact function_beta_expansion f h0 h2
+  have ⟨eam,h3,h4⟩ := h0 e' h2
+  have h5 := Typing.soundness h2
+  apply Typing.function_beta_expansion f .hole h5 h3 h4
 
 theorem Typing.function_preservation {am p tp e f t } :
   (∀ {v} , Expr.is_value v → Typing am v tp → ∃ eam , Expr.pattern_match v p = .some eam) →
