dsn/Lang/Dynamic/Safe.lean
@@ -1,0 +1,220 @@
+import Lang.Basic
+import Lang.Dynamic.EvalCon
+import Lang.Dynamic.Transition
+import Lang.Dynamic.TransitionStar
+
+set_option pp.fieldNotation false
+
+
+namespace Lang.Dynamic
+
+
+def Convergent (e : Expr) : Prop :=
+  ∃ e' , TransitionStar e e' ∧ Expr.is_value e'
+
+mutual
+
+  theorem Convergent.subject_reduction
+    (transition : Transition e e')
+  : Convergent e → Convergent e'
+  := by sorry
+
+  theorem Convergent.subject_expansion
+    (transition : Transition e e')
+  : Convergent e' → Convergent e
+  := by sorry
+
+end
+
+
+theorem Convergent.econ_reflection :
+  EvalCon E →
+  Convergent (E e) →
+  Convergent e
+:= by
+  sorry
+
+theorem Convergent.econ_preservation :
+  EvalCon E → Convergent (E e) →
+  Convergent e' → Convergent (E e')
+:= by sorry
+
+
+
+mutual
+  theorem Convergent.record_beta_reduction :
+    EvalCon E →
+    Convergent (E (Expr.project (Expr.record [(l, e)]) l)) →
+    Convergent (E e)
+  := by sorry
+
+  theorem Convergent.record_beta_expansion l :
+    EvalCon E →
+    Convergent (E e) →
+    Convergent (E (Expr.project (Expr.record [(l, e)]) l))
+  := by sorry
+end
+
+mutual
+  theorem Convergent.function_beta_reduction
+    (econ : EvalCon E)
+    (isval : Expr.is_value ev)
+    (matching : Expr.pattern_match ev p = .some eam)
+  : Convergent (E (Expr.app (Expr.function ((p, e) :: f)) ev)) →
+    Convergent (E (Expr.sub eam e))
+  := by sorry
+
+  theorem Convergent.function_beta_expansion f
+    (econ : EvalCon E)
+    (isval : Expr.is_value ev)
+    (matching : Expr.pattern_match ev p = .some eam)
+  : Convergent (E (Expr.sub eam e)) →
+    Convergent (E (Expr.app (Expr.function ((p, e) :: f)) ev))
+  := by sorry
+end
+
+def Divergent (e : Expr) : Prop :=
+  (∀ e', TransitionStar e e' → ∃ e'' , Transition e' e'')
+
+
+mutual
+
+  theorem Divergent.subject_reduction
+    (transition : Transition e e')
+  : Divergent e → Divergent e'
+  := by sorry
+
+  theorem Divergent.subject_expansion
+    (transition : Transition e e')
+  : Divergent e' → Divergent e
+  := by sorry
+
+end
+
+theorem Divergent.econ_preservation :
+  EvalCon E →
+  Divergent e →
+  Divergent (E e)
+:= by
+  sorry
+
+theorem Divergent.econ_reflection :
+  EvalCon E →
+  Divergent (E e) →
+  Divergent e
+:= by
+  sorry
+
+
+-- theorem Divergent.swap_preservation
+--   (econ : EvalCon E)
+--   (isval : Expr.is_value e)
+--   (dvg_econ : Divergent (E e))
+-- : Divergent (E e')
+-- := by sorry
+
+mutual
+  theorem Divergent.record_beta_reduction :
+    EvalCon E →
+    Divergent (E (Expr.project (Expr.record [(l, e)]) l)) →
+    Divergent (E e)
+  := by sorry
+
+  theorem Divergent.record_beta_expansion l :
+    EvalCon E →
+    Divergent (E e) →
+    Divergent (E (Expr.project (Expr.record [(l, e)]) l))
+  := by sorry
+end
+
+mutual
+  theorem Divergent.function_beta_reduction
+    (econ : EvalCon E)
+    (isval : Expr.is_value ev)
+    (matching : Expr.pattern_match ev p = .some eam)
+  : Divergent (E (Expr.app (Expr.function ((p, e) :: f)) ev)) →
+    Divergent (E (Expr.sub eam e))
+  := by sorry
+
+  theorem Divergent.function_beta_expansion f
+    (econ : EvalCon E)
+    (isval : Expr.is_value ev)
+    (matching : Expr.pattern_match ev p = .some eam)
+  : Divergent (E (Expr.sub eam e)) →
+    Divergent (E (Expr.app (Expr.function ((p, e) :: f)) ev))
+  := by sorry
+end
+
+
+
+
+
+
+
+
+
+def Safe (e : Expr) : Prop := Convergent e ∨ Divergent e
+
+mutual
+
+  theorem Safe.subject_reduction
+    (transition : Transition e e')
+  : Safe e → Safe e'
+  := by sorry
+
+  theorem Safe.subject_expansion
+    (transition : Transition e e')
+  : Safe e' → Safe e
+  := by sorry
+
+end
+
+
+theorem Safe.econ_reflection :
+  EvalCon E →
+  Safe (E e) →
+  Safe e
+:= by
+  sorry
+
+theorem Safe.econ_preservation :
+  EvalCon E → Safe (E e) →
+  Safe e' → Safe (E e')
+:= by sorry
+
+
+
+mutual
+  theorem Safe.record_beta_reduction :
+    EvalCon E →
+    Safe (E (Expr.project (Expr.record [(l, e)]) l)) →
+    Safe (E e)
+  := by sorry
+
+  theorem Safe.record_beta_expansion l :
+    EvalCon E →
+    Safe (E e) →
+    Safe (E (Expr.project (Expr.record [(l, e)]) l))
+  := by sorry
+end
+
+mutual
+  theorem Safe.function_beta_reduction
+    (econ : EvalCon E)
+    (safe_arg : Safe arg)
+    (matching : Expr.pattern_match ev p = .some eam)
+  : Safe (E (Expr.app (Expr.function ((p, e) :: f)) arg)) →
+    Safe (E (Expr.sub eam e))
+  := by sorry
+
+  theorem Safe.function_beta_expansion f
+    (econ : EvalCon E)
+    (safe_arg : Safe arg)
+    (matching : Expr.pattern_match ev p = .some eam)
+  : Safe (E (Expr.sub eam e)) →
+    Safe (E (Expr.app (Expr.function ((p, e) :: f)) arg))
+  := by sorry
+end
+
+
+end Lang.Dynamic
