dsn/Lang/Static.lean
@@ -2829,6 +2829,7 @@ mutual
       apply Typing.path_intro
       intros v p44 p46
       have ⟨eam0,p48,p50⟩ := PatLifting.Static.soundness pat_lifting_static (tam0 ++ tam') v p44 p46
+
       exists eam0
       simp [*]
       rw [Expr.sub_sub_removal (pattern_match_ids_containment p48)]
